Woohoo, tests restored with tactics and everything, needs protz_misc branch for F* at the moment

providers/test/Test.fst
@@ -16,140 +16,176 @@ module AC = EverCrypt.AutoConfig
 module H = EverCrypt.Hash
 
 open Test.Vectors
-open FStar.Integers
 open LowStar.BufferOps
 
 #set-options "--admit_smt_queries true"
 
 /// Hash function (any of them)
 
-val test_one_hash: v:hash_vector -> St unit
-let test_one_hash v =
-  push_frame();
+let vec8 = B.buffer UInt8.t * UInt32.t
+let hash_vector = hash_alg * C.String.t * vec8 * UInt32.t
 
-  let output_len: UInt32.t =
-    match v.hash_alg with
-    | H.SHA256 -> 32ul
-    | H.SHA384 -> 48ul
-    //| H.SHA512 -> 64ul
-  in
-  let output = B.alloca 0uy output_len in
+noextract unfold inline_for_extraction let (!$) = C.String.((!$))
 
-  let input_len = C.String.strlen v.input in
-  let total_input_len = input_len * v.repeat in
-  let input = B.alloca 0uy total_input_len in
-  C.Loops.for 0ul v.repeat (fun _ _ -> True) (fun i ->
-    C.String.memcpy (B.offset input (input_len * i)) v.input input_len
-  );
+open C.Failure
 
-  (* Allocate memory for state *)
-  let ctx = EverCrypt.Hash.(create v.hash_alg) in
+let supported_hash_algorithm = function
+  | SHA256 | SHA384 -> true
+  | _ -> false
 
-  (* Compute the number of blocks to process *)
-  let size_block: UInt32.t =
-    match v.hash_alg with
-    | H.SHA256 -> 64ul
-    | H.SHA384 -> 128ul
-    //| SHA512 -> 128ul
-  in
-  let n = U32.div total_input_len size_block in
-  let r = U32.rem total_input_len size_block in
+let as_alg = function
+  | SHA256 -> H.SHA256
+  | SHA384 -> H.SHA384
+  | _ -> failwith !$"unsupported alg"
 
-  (* Get all full blocks and the last block *)
-  let input_blocks = B.sub input 0ul (n * size_block) in
-  let input_last   = B.sub input (n * size_block) r in
+val test_one_hash: hash_vector -> St unit
+let test_one_hash vec =
+  let open FStar.Integers in
+  let hash_alg, input, (output, output_len), repeat = vec in
 
-  (* Call the hash function incrementally *)
-  EverCrypt.Hash.init ctx;
-  EverCrypt.Hash.update_multi ctx input_blocks n;
-  EverCrypt.Hash.update_last ctx input_last r;
-  EverCrypt.Hash.finish ctx output;
+  if supported_hash_algorithm hash_alg then begin
 
-  // Non-incrementally:
-  // EverCrypt.sha256_hash output input len
+    push_frame();
 
-  let str: C.String.t =
-    match v.hash_alg with
-    | H.SHA256 -> !$"of SHA256"
-    | H.SHA384 -> !$"of SHA384"
-  in
+    let output_len: UInt32.t =
+      match hash_alg with
+      | SHA256 -> 32ul
+      | SHA384 -> 48ul
+      | _ -> failwith !$"Unsupported algorithm"
+    in
+    let output = B.alloca 0uy output_len in
 
-  (* Display the result *)
-  TestLib.compare_and_print str !!v.output !!output output_len;
+    let input_len = C.String.strlen input in
+    let total_input_len = input_len * repeat in
+    let total_input = B.alloca 0uy total_input_len in
+    C.Loops.for 0ul repeat (fun _ _ -> True) (fun i ->
+      C.String.memcpy (B.offset total_input (input_len * i)) input input_len
+    );
 
-  pop_frame()
+    (* Allocate memory for state *)
+    let a: H.alg = as_alg hash_alg in
+    let ctx = EverCrypt.Hash.create a in
+
+    (* Compute the number of blocks to process *)
+    let size_block: UInt32.t =
+      match hash_alg with
+      | SHA256 -> 64ul
+      | SHA384 -> 128ul
+      | _ -> failwith !$"Unsupported algorithm"
+    in
+    let n = U32.div total_input_len size_block in
+    let r = U32.rem total_input_len size_block in
+
+    (* Get all full blocks and the last block *)
+    let input_blocks = B.sub total_input 0ul (n * size_block) in
+    let input_last   = B.sub total_input (n * size_block) r in
+
+    (* Call the hash function incrementally *)
+    EverCrypt.Hash.init ctx;
+    EverCrypt.Hash.update_multi ctx input_blocks n;
+    EverCrypt.Hash.update_last ctx input_last r;
+    EverCrypt.Hash.finish ctx output;
+
+    // Non-incrementally:
+    // EverCrypt.sha256_hash output input len
+
+    let str: C.String.t =
+      match hash_alg with
+      | SHA256 -> !$"of SHA256"
+      | SHA384 -> !$"of SHA384"
+    in
+
+    (* Display the result *)
+    TestLib.compare_and_print str !!output !!output output_len;
+
+    pop_frame()
+  end
 
 /// ChaCha20-Poly1305
 
-val test_chacha20_poly1305: v:aead_vector{v.cipher == CHACHA20_POLY1305} -> St unit
-let test_chacha20_poly1305 v =
+let aead_vector = cipher * vec8 * vec8 * vec8 * vec8 * vec8 * vec8
+
+val test_chacha20_poly1305: aead_vector -> St unit
+let test_chacha20_poly1305 vec =
   push_frame();
 
-  let plaintext'    = B.alloca 0uy v.plaintext_len in
-  let ciphertext'   = B.alloca 0uy v.plaintext_len in
+  let cipher, (key, key_len), (iv, iv_len), (aad, aad_len),
+    (tag, tag_len), (plaintext, plaintext_len), (ciphertext, ciphertext_len) = vec
+  in
+
+  let plaintext'    = B.alloca 0uy plaintext_len in
+  let ciphertext'   = B.alloca 0uy plaintext_len in
   let tag'          = B.alloca 0uy 16ul in
 
   let s0 = TestLib.cpucycles () in
-  EverCrypt.chacha20_poly1305_encrypt v.key v.iv v.aad v.aad_len v.plaintext v.plaintext_len ciphertext' tag';
+  EverCrypt.chacha20_poly1305_encrypt key iv aad aad_len plaintext plaintext_len ciphertext' tag';
   let s1 = TestLib.cpucycles () in
   TestLib.print_cycles_per_round s0 s1 1ul;
-  TestLib.compare_and_print !$"of Chacha20-Poly1305 cipher" !!v.ciphertext !!ciphertext' v.plaintext_len;
-  TestLib.compare_and_print !$"of Chacha20-Poly1305 tag" !!v.tag !!tag' 16ul;
+  TestLib.compare_and_print !$"of Chacha20-Poly1305 cipher" !!ciphertext !!ciphertext' plaintext_len;
+  TestLib.compare_and_print !$"of Chacha20-Poly1305 tag" !!tag !!tag' 16ul;
 
-  match EverCrypt.chacha20_poly1305_decrypt v.key v.iv v.aad v.aad_len plaintext' v.plaintext_len v.ciphertext v.tag with
+  match EverCrypt.chacha20_poly1305_decrypt key iv aad aad_len plaintext' plaintext_len ciphertext tag with
   | 1ul ->
-    TestLib.compare_and_print !$"of Chacha20-Poly1305 plaintext" !!v.plaintext !!plaintext' v.plaintext_len
+    TestLib.compare_and_print !$"of Chacha20-Poly1305 plaintext" !!plaintext !!plaintext' plaintext_len
   | _ ->
     C.String.print !$"Decryption failed!\n"; C.portable_exit 1l;
 
   pop_frame()
 
-val test_aes128_gcm: v:aead_vector{v.cipher == AES_128_GCM} -> St unit
-let test_aes128_gcm v =
+val test_aes128_gcm: v:aead_vector -> St unit
+let test_aes128_gcm vec =
   push_frame();
 
-  let plaintext'    = B.alloca 0uy v.plaintext_len in
-  let ciphertext'   = B.alloca 0uy v.plaintext_len in
+  let cipher, (key, key_len), (iv, iv_len), (aad, aad_len),
+    (tag, tag_len), (plaintext, plaintext_len), (ciphertext, ciphertext_len) = vec
+  in
+
+  let plaintext'    = B.alloca 0uy plaintext_len in
+  let ciphertext'   = B.alloca 0uy plaintext_len in
   let tag'          = B.alloca 0uy 16ul in
 
   let s0 = TestLib.cpucycles () in
-  EverCrypt.aes128_gcm_encrypt v.key v.iv v.aad v.aad_len v.plaintext v.plaintext_len ciphertext' tag';
+  EverCrypt.aes128_gcm_encrypt key iv aad aad_len plaintext plaintext_len ciphertext' tag';
   let s1 = TestLib.cpucycles () in
   TestLib.print_cycles_per_round s0 s1 1ul;
-  TestLib.compare_and_print !$"of AES-GCM 128 cipher" !!v.ciphertext !!ciphertext' v.plaintext_len;
-  TestLib.compare_and_print !$"of AES-GCM 128 tag" !!v.tag !!tag' 16ul;
+  TestLib.compare_and_print !$"of AES-GCM 128 cipher" !!ciphertext !!ciphertext' plaintext_len;
+  TestLib.compare_and_print !$"of AES-GCM 128 tag" !!tag !!tag' 16ul;
 
-  match EverCrypt.aes128_gcm_decrypt v.key v.iv v.aad v.aad_len plaintext' v.plaintext_len v.ciphertext v.tag with
+  match EverCrypt.aes128_gcm_decrypt key iv aad aad_len plaintext' plaintext_len ciphertext tag with
   | 1ul ->
-    TestLib.compare_and_print !$"of AES-GCM 128 plaintext" !!v.plaintext !!plaintext' v.plaintext_len
+    TestLib.compare_and_print !$"of AES-GCM 128 plaintext" !!plaintext !!plaintext' plaintext_len
   | _ ->
     C.String.print !$"Decryption failed!\n"; C.portable_exit 1l;
 
   pop_frame()
 
-val test_aes256_gcm: v:aead_vector{v.cipher == AES_256_GCM} -> St unit
-let test_aes256_gcm v =
+val test_aes256_gcm: v:aead_vector -> St unit
+let test_aes256_gcm vec =
   push_frame();
 
-  let plaintext'    = B.alloca 0uy v.plaintext_len in
-  let ciphertext'   = B.alloca 0uy v.plaintext_len in
+  let cipher, (key, key_len), (iv, iv_len), (aad, aad_len),
+    (tag, tag_len), (plaintext, plaintext_len), (ciphertext, ciphertext_len) = vec
+  in
+
+  let plaintext'    = B.alloca 0uy plaintext_len in
+  let ciphertext'   = B.alloca 0uy plaintext_len in
   let tag'          = B.alloca 0uy 16ul in
 
-  EverCrypt.aes256_gcm_encrypt v.key v.iv v.aad v.aad_len v.plaintext v.plaintext_len ciphertext' tag';
-  TestLib.compare_and_print !$"of AES-GCM 256 cipher" !!v.ciphertext !!ciphertext' v.plaintext_len;
-  TestLib.compare_and_print !$"of AES-GCM 256 tag" !!v.tag !!tag' 16ul;
+  EverCrypt.aes256_gcm_encrypt key iv aad aad_len plaintext plaintext_len ciphertext' tag';
+  TestLib.compare_and_print !$"of AES-GCM 256 cipher" !!ciphertext !!ciphertext' plaintext_len;
+  TestLib.compare_and_print !$"of AES-GCM 256 tag" !!tag !!tag' 16ul;
 
   let s0 = TestLib.cpucycles () in
-  EverCrypt.aes256_gcm_encrypt v.key v.iv v.aad v.aad_len v.plaintext v.plaintext_len ciphertext' tag';
+  EverCrypt.aes256_gcm_encrypt key iv aad aad_len plaintext plaintext_len ciphertext' tag';
   let s1 = TestLib.cpucycles () in
 
   TestLib.print_cycles_per_round s0 s1 1ul;
-  TestLib.compare_and_print !$"of AES-GCM 256 cipher" !!v.ciphertext !!ciphertext' v.plaintext_len;
-  TestLib.compare_and_print !$"of AES-GCM 256 tag" !!v.tag !!tag' 16ul;
+  TestLib.compare_and_print !$"of AES-GCM 256 cipher" !!ciphertext !!ciphertext' plaintext_len;
+  TestLib.compare_and_print !$"of AES-GCM 256 tag" !!tag !!tag' 16ul;
 
-  match EverCrypt.aes256_gcm_decrypt v.key v.iv v.aad v.aad_len plaintext' v.plaintext_len v.ciphertext v.tag with
+  match EverCrypt.aes256_gcm_decrypt key iv aad aad_len plaintext' plaintext_len ciphertext tag with
   | 1ul ->
-    TestLib.compare_and_print !$"of AES-GCM 256 plaintext" !!v.plaintext !!plaintext' v.plaintext_len
+    TestLib.compare_and_print !$"of AES-GCM 256 plaintext" !!plaintext !!plaintext' plaintext_len
   | _ ->
     C.String.print !$"Decryption failed!\n"; C.portable_exit 1l;
 
@@ -214,20 +250,22 @@ let rec test_aead len vs =
     ()
   else
     let v = vs.(0ul) in
-    begin match v.cipher with
-    | CHACHA20_POLY1305 ->
+    begin match v with
+    | CHACHA20_POLY1305, _, _, _, _, _, _ ->
         test_chacha20_poly1305 v
-    | AES_128_GCM ->
+    | AES_128_GCM, _, _, _, _, _, _ ->
         () // JP: TODO: FIXME // test_aes128_gcm v
-    | AES_256_GCM ->
+    | AES_256_GCM, _, _, _, _, _, _ ->
         () // JP: TODO: FIXME // test_aes256_gcm v
     | _ ->
         ()
     end;
+    let open FStar.Integers in
     test_aead (len - 1ul) (B.offset vs 1ul)
 
 val test_hash: len:U32.t -> vs: B.buffer hash_vector {B.len vs = len }-> St unit
 let rec test_hash len vs =
+  let open FStar.Integers in
   if len > 0ul then
     let v = vs.(0ul) in
     test_one_hash v;
@@ -237,6 +275,9 @@ let main (): St C.exit_code =
   let open EverCrypt in
   let open C.String in
   push_frame ();
+
+  let hash_vectors, hash_vectors_len = hash_vectors_low in
+  let aead_vectors, aead_vectors_len = aead_vectors_low in
 
   print !$"===========Hacl===========";
   AC.(init (Prefer Hacl));
